Add comments and introduce 'satisfies'

BoltLean/Boolean/Basic.lean
@@ -1,17 +1,21 @@
-abbrev Valuation (n_var: Nat): Type := Vector Bool n_var
+/-- A valuation represents the membership of a given element `x` of the universe
+in each of the sets `S_1, ..., S_{n_sets}` of the instance.
+It is an alias for `Vector Bool n_sets`,
+and `v[i]` says whether `x` is in `S_i`.-/
+abbrev Valuation (n_sets: Nat): Type := Vector Bool n_sets
 
 /- Boolean formulas in NNF -/
-inductive BoolFormula (n_var: Nat)
-  | False: BoolFormula n_var
-  | True : BoolFormula n_var
-  | Var : Fin n_var -> (neg: Bool) -> BoolFormula n_var
-  | And : BoolFormula n_var -> BoolFormula n_var -> BoolFormula n_var
-  | Or : BoolFormula n_var -> BoolFormula n_var -> BoolFormula n_var
+inductive BoolFormula (n_sets: Nat)
+  | False: BoolFormula n_sets
+  | True : BoolFormula n_sets
+  | Var : Fin n_sets -> (neg: Bool) -> BoolFormula n_sets
+  | And : BoolFormula n_sets -> BoolFormula n_sets -> BoolFormula n_sets
+  | Or : BoolFormula n_sets -> BoolFormula n_sets -> BoolFormula n_sets
   deriving DecidableEq, Repr
 
 namespace BoolFormula
   @[simp]
-  def accepts (f: BoolFormula n_var) (v: Valuation n_var): Prop :=
+  def accepts (f: BoolFormula n_sets) (v: Valuation n_sets): Prop :=
     match f with
     | False => _root_.False
     | True => _root_.True
@@ -19,10 +23,19 @@ namespace BoolFormula
     | And f1 f2 => f1.accepts v ∧ f2.accepts v
     | Or f1 f2 => f1.accepts v ∨ f2.accepts v
 
-  def dominates (f1 f2: BoolFormula n_var): Prop :=
-    ∀ (v: Valuation n_var), f2.accepts v → f1.accepts v
+  /-- A formula satisfies an examples if it is positive and the formula accepts,
+  or if it is negative and the formula rejects.-/
+  @[simp]
+  def satisfies (f: BoolFormula n_sets) (v: Valuation n_sets) (positive: Bool) : Prop :=
+    f.accepts v ↔ positive
 
-  def replace (f pat repl: BoolFormula n_var): BoolFormula n_var :=
+  /-- A formula `f1` dominates `f2` another if `f1` satisfies a superset
+  of the elements satisfied by `f2`.-/
+  def dominates (f1 f2: BoolFormula n_sets): Prop :=
+    ∀ (v: Valuation n_sets) (b: Bool), f2.satisfies v b → f1.satisfies v b
+
+  /-- Replace all occurrence of the formula `pat` in `f` with the formula `repl`.-/
+  def replace (f pat repl: BoolFormula n_sets): BoolFormula n_sets :=
     if f = pat then
       repl
     else match f with
