BoltLean/Boolean/Domination.lean
@@ -1,21 +1,36 @@
 import BoltLean.Boolean.Basic
 
 namespace BoolFormula
-  theorem true_replace_accepts (f1 f2: BoolFormula n_var):
-    f1.dominates f2 -> ∀ (v: Valuation n_var), (True.replace f2 f1).accepts v := by
+  /-- Aux Lemma: `True` -/
+  theorem true_replace_accepts (f1 f2: BoolFormula n):
+    f1.dominates f2 -> ∀ (v: Valuation n), (True.replace f2 f1).accepts v := by
       intro h v
       simp [replace]
       split
       . next heq =>
           rw [←heq] at h
+          simp [dominates] at h
           apply h
-          simp
       . next hne => simp
 
+  /-- Aux Lemma: `False` -/
+  theorem false_replace_not_accepts (f1 f2: BoolFormula n):
+    f1.dominates f2 -> ∀ (v: Valuation n), ¬ (False.replace f2 f1).accepts v := by
+      intro h v
+      simp [replace]
+      split
+      . next heq =>
+          rw [←heq] at h
+          simp [dominates] at h
+          apply h
+      . next hne => simp
 
-  theorem var_replace_accepts (f1 f2: BoolFormula n_var) (i: Fin n_var) (neg: Bool):
-    f1.dominates f2 -> ∀ (v: Valuation n_var), (Var i neg).accepts v -> ((Var i neg).replace f2 f1).accepts v := by
-      intro h v hv
+  /-- Aux Lemma: `Var` -/
+  theorem var_replace_accepts (f1 f2: BoolFormula n) (i: Fin n) (neg: Bool):
+    f1.dominates f2 ->
+      ∀ (v: Valuation n) (b: Bool),
+        (Var i neg).satisfies v b -> ((Var i neg).replace f2 f1).satisfies v b := by
+      intro h v b hv
       simp [replace]
       split
       . next heq =>
@@ -24,13 +39,21 @@ namespace BoolFormula
           exact hv
       . next hne => assumption
 
-  theorem domin_replace (f1 f2: BoolFormula n_var):
+  /-- Theorem: if f1 dominates f2, then in any formula f,
+  replacing f2 by f1 yields a dominating formula.-/
+  theorem domin_replace (f1 f2: BoolFormula n):
     f1.dominates f2 →
-      ∀ (f: BoolFormula n_var), (f.replace f2 f1).dominates f := by
-      intro hd f v ha
+      ∀ (f: BoolFormula n), (f.replace f2 f1).dominates f := by
+      intro hd f v b ha
       induction f with
-      | True => exact true_replace_accepts f1 f2 hd v
-      | False => contradiction
+      | True =>
+        cases b with
+        | false => simp at ha
+        | true => simp; exact true_replace_accepts f1 f2 hd v
+      | False =>
+        cases b with
+        | false => simp [replace]; exact false_replace_not_accepts f1 f2 hd v
+        | true => simp at ha
       | Var i neg =>
         apply var_replace_accepts
           <;> assumption
@@ -38,27 +61,37 @@ namespace BoolFormula
         simp [replace]
         split
         . next heq =>
-          rw [←heq] at hd
-          apply hd v
-          assumption
+          apply hd
+          rw [heq] at ha
+          exact ha
         . next hne =>
-          simp
-          simp at ha
-          constructor
-          . exact ih1 ha.left
-          . exact ih2 ha.right
+          cases b with
+          | false =>
+            simp at *
+            intro h
+            by_cases hx: g1.accepts v
+            . exact ih2 (ha hx)
+            . have hc:= ih1 hx
+              contradiction
+          | true =>
+            simp at *
+            exact ⟨ih1 ha.left, ih2 ha.right⟩
       | Or g1 g2 ih1 ih2 =>
         simp [replace]
         split
         . next heq =>
-          rw [←heq] at hd
-          apply hd v
+          apply hd
+          rw [heq] at ha
           assumption
         . next hne =>
-          simp
-          simp at ha
-          match ha with
-          | .inl h1 => left; exact ih1 h1
-          | .inr h2 => right; exact ih2 h2
+          cases b with
+          | false =>
+            simp at *
+            exact ⟨ih1 ha.left, ih2 ha.right⟩
+          | true =>
+            simp at *
+            match ha with
+            | .inl h1 => left; exact ih1 h1
+            | .inr h2 => right; exact ih2 h2
 
 end BoolFormula
