BoltLean/Ltl/Basic.lean
@@ -1,10 +1,13 @@
+/-- `Trace n_pred` is an alias for `List (Vector Bool n_pred)`.
+At position `i` in the list, the vector contains the truth value of the `n_pred` predicates at time `i`.-/
 abbrev Trace (n_pred: Nat): Type := List (Vector Bool n_pred)
 
 /-- LTL Formulas in NNF -/
 inductive Formula n_pred
   | True : Formula n_pred
   | False : Formula n_pred
-  | Var : Fin n_pred -> (neg: Bool) -> Formula n_pred -- neg: Whether the variable is negated
+  /-- neg: Whether the variable is negated -- negations are only allowed at variables. -/
+  | Var : Fin n_pred -> (neg: Bool) -> Formula n_pred
   | Next : Formula n_pred -> Formula n_pred
   | WeakNext : Formula n_pred -> Formula n_pred
   | Globally : Formula n_pred -> Formula n_pred
@@ -15,9 +18,11 @@ inductive Formula n_pred
 deriving DecidableEq
 
 namespace Formula
-
+  /-- Whether the formula is satisfied by the Trace.-/
   def accepts (phi: Formula n) (t: Trace n): Prop :=
   match t with
+    -- Special case of the empty Trace: it is only accepted by True and Globally,
+    -- or their boolean combinations.
     | .nil => match phi with
       | True | Globally _ => _root_.True
       | False | Finally _ | Var _ _ | Next _ | WeakNext _ | Until _ _ => _root_.False
@@ -36,7 +41,5 @@ namespace Formula
       | Until psi1 psi2 => ∃ j, j < t.length ∧
                                 (accepts psi2 (t.drop j)) ∧
                                 (∀ k, k < j → accepts psi1 (t.drop k))
-
-  def equivalence (phi psi : Formula n) : Prop := ∀ (t : Trace n), accepts phi t ↔ accepts psi t
 
 end Formula
